XOR is now a function

src/xor/direct_xor.lean
@@ -1,6 +1,6 @@
 /-
-This file defines and proves the equisatisfiability of the direct (or naive)
-encoding for the n-variable XOR gate.
+This file defines and proves the correctness of the direct (or naive)
+encoding of the n-variable boolean XOR function.
 
 Authors: Cayden Codel, Jeremy Avigad, Marijn Heule
 Carnegie Mellon University
@@ -18,7 +18,7 @@ import data.nat.basic
 
 universe u
 
--- Represents the parametric type of the variable stored in the literal
+-- Represents the type of the variable stored in the literal
 variables {V : Type u} [decidable_eq V] [inhabited V]
 
 namespace Xor
@@ -34,24 +34,25 @@ open nat
 /-! # Direct encoding -/
 section direct_encoding
 
-variables {g : Xor V} {c : clause V}
+variables {l : list (literal V)} {c : clause V}
 
 /- The direct encoding is the set of all possible clauses with an even number 
    of negations on the provided literals in a single CNF formula. -/
-def direct_xor : Xor V → cnf V
+def direct_xor : list (literal V) → cnf V
 | []        := [[]]
 | (l :: ls) := (explode (map var ls)).map 
       (λ c, ite (!bodd (c.count_flips ls)) (l :: c) (l.flip :: c))
 
-@[simp] theorem direct_xor_nil : direct_xor ([] : Xor V) = [[]] := rfl
+@[simp] theorem direct_xor_nil : direct_xor ([] : list (literal V)) = [[]] := rfl
 
-@[simp] theorem direct_xor_singleton (l : literal V) : direct_xor [l] = [[l]] :=
+@[simp] theorem direct_xor_singleton (lit : literal V) : 
+  direct_xor [lit] = [[lit]] :=
 by simp [direct_xor]
 
 theorem mem_explode_of_mem_direct_xor : 
-  c ∈ direct_xor g → c ∈ explode (map var g) :=
+  c ∈ direct_xor l → c ∈ explode (map var l) :=
 begin
-  cases g with l ls,
+  cases l with l ls,
   { simp only [explode_nil, imp_self, direct_xor_nil, map_nil] },
   { simp [direct_xor, explode],
     intros cl hcl,
@@ -66,21 +67,21 @@ begin
         use [cl, hcl, h] } } }
 end
 
-theorem length_direct_xor : g ≠ [] → length (direct_xor g) = 2^(length g - 1) :=
+theorem length_direct_xor : l ≠ [] → length (direct_xor l) = 2^(length l - 1) :=
 begin
-  cases g,
+  cases l,
   { contradiction },
   { simp only [direct_xor, length_explode, add_zero, length, add_succ_sub_one, 
       ne.def, forall_true_left, not_false_iff, length_map] }
 end
 
-theorem length_direct_xor_pos : g ≠ [] → length (direct_xor g) > 0 :=
+theorem length_direct_xor_pos : l ≠ [] → length (direct_xor l) > 0 :=
 assume h, by simp only [length_direct_xor h, succ_pos', gt_iff_lt, pow_pos]
 
-theorem exists_mem_direct_xor (g : Xor V) : 
-  ∃ (c : clause V), c ∈ direct_xor g :=
+theorem exists_mem_direct_xor (l : list (literal V)) : 
+  ∃ (c : clause V), c ∈ direct_xor l :=
 begin
-  cases g with l ls,
+  cases l with l ls,
   { use [nil, mem_singleton_self nil] },
   { exact exists_mem_of_length_pos (length_direct_xor_pos (cons_ne_nil l ls)) }
 end
@@ -88,9 +89,9 @@ end
 -- These theorems begin to be dependent on order of encoding
 -- If the underlying type of Xor changes to (fin)set, must update
 theorem map_var_eq_of_mem_direct_xor :
-  c ∈ direct_xor g → map var c = map var g :=
+  c ∈ direct_xor l → map var c = map var l :=
 begin
-  cases g with l ls,
+  cases l with l ls,
   { simp only [direct_xor, imp_self, map_eq_nil, map_nil, mem_singleton] },
   { simp [direct_xor],
     intros c hc,
@@ -103,11 +104,11 @@ begin
       simp [map_var_eq_iff_mem_explode.mpr hc, flip_var_eq] } }
 end
 
-theorem even_flips_iff_mem_direct_xor_of_map_var_eq : map var c = map var g → 
-  (bodd (c.count_flips g) = ff ↔ c ∈ direct_xor g) :=
+theorem even_flips_iff_mem_direct_xor_of_map_var_eq : map var c = map var l → 
+  (bodd (c.count_flips l) = ff ↔ c ∈ direct_xor l) :=
 begin
   intro hc, split,
-  { cases g with l ls,
+  { cases l with l ls,
     { revert hc, simp },
     { simp only [direct_xor, map_cons, bool.cond_to_bool, mem_map],
       intro hf,
@@ -123,7 +124,7 @@ begin
           { simp [clause.count_flips, hx] at hf,
             rw h at hf, contradiction },
           { simp only [flip_flip, if_false, bool.bnot_true, coe_sort_ff]} } } } },
-  { cases g with l ls,
+  { cases l with l ls,
     { simp },
     { simp only [direct_xor, bool.cond_to_bool, mem_map],
       rintro ⟨a, ha, hf⟩,
@@ -134,8 +135,8 @@ begin
           bool.to_nat, h, flip_flip _, flip_ne] } } }      
 end
 
-theorem odd_flips_iff_not_mem_direct_xor_of_map_var_eq : map var c = map var g → 
-  (bodd (c.count_flips g) = tt ↔ c ∉ direct_xor g) :=
+theorem odd_flips_iff_not_mem_direct_xor_of_map_var_eq : map var c = map var l → 
+  (bodd (c.count_flips l) = tt ↔ c ∉ direct_xor l) :=
 begin
   intro hc, split,
   { intro hcount, by_contradiction,
@@ -145,19 +146,19 @@ begin
     exact (even_flips_iff_mem_direct_xor_of_map_var_eq hc).mp }
 end
 
-theorem mem_direct_xor_self (g : Xor V) : g ∈ (direct_xor g) :=
+theorem mem_direct_xor_self (l : list (literal V)) : l ∈ (direct_xor l) :=
 begin
-  have hcount := clause.count_flips_self g,
+  have hcount := clause.count_flips_self l,
   have := nat.bodd_zero,
   rw ← hcount at this,
   exact (even_flips_iff_mem_direct_xor_of_map_var_eq (refl _)).mp this
 end
 
 -- Some proofs require the stronger statement that direct is exactly xor
-theorem eval_direct_xor_eq_eval_Xor (g : Xor V) (τ : assignment V) :
-  (direct_xor g).eval τ = g.eval τ :=
+theorem eval_direct_xor_eq_eval_Xor (l : list (literal V)) (τ : assignment V) :
+  (direct_xor l).eval τ = Xor.eval τ l :=
 begin
-  cases g with l ls,
+  cases l with l ls,
   { simp only [cnf.eval_singleton, eval_nil, direct_xor_nil, clause.eval_nil] },
   { have he := eval_eq_bodd_count_tt τ (l :: ls),
     cases h : (Xor.eval τ (l :: ls)),
@@ -182,16 +183,15 @@ begin
       exact clause.eval_tt_of_ne_flips mve.symm (ne.symm neq) } }
 end
 
-theorem vars_direct_xor (g : Xor V) : (direct_xor g).vars = g.vars :=
+theorem vars_direct_xor (l : list (literal V)) : 
+  (direct_xor l).vars = clause.vars l :=
 begin
-  cases g with l ls,
-  { simp only [cnf.vars_singleton, direct_xor_nil, vars_nil, clause.vars_nil] },
-  { rw finset.ext_iff,
-    intro v,
-    split,
+  cases l with l ls,
+  { simp only [cnf.vars_singleton, direct_xor_nil] },
+  { rw finset.ext_iff, intro v, split,
     { intro hv,
       rcases mem_vars_iff_exists_mem_clause_and_mem.mp hv with ⟨c, hc⟩,
-      rw [vars, clause.mem_vars_iff_mem_map_vars],
+      rw [clause.mem_vars_iff_mem_map_vars],
       rw ← (map_var_eq_of_mem_direct_xor hc.1),
       exact clause.mem_vars_iff_mem_map_vars.mp hc.2 },
     { intro hv,
