src/xor/xor.lean
@@ -1,6 +1,5 @@
 /-
-This file defines the XOR gate on n variables, as well as
-general properties of evaluation of XORs.
+This file defines the boolean XOR function on n variables.
 
 Authors: Cayden Codel, Marijn Heule, Jeremy Avigad
 Carnegie Mellon University
@@ -18,15 +17,11 @@ import data.finset.basic
 
 universe u
 
--- Represents the parametric type of the variable stored in the literal
+-- Represents the type of the variable stored in the literal
 variables {V : Type u} [decidable_eq V] [inhabited V]
 
-/- An n-literal XOR function is a list of those literals. -/
--- Unfortunately, "xor" was already defined, so "n"xor to mean n literals
-def Xor (V : Type u) := list (literal V)
-
--- Not to be confused with the XNOR gate
--- See the note in cnf/clause.lean for discussion of list vs. set typing
+/- An n-variable XOR function is a map from a list of bools to an output bool -/
+def Xor (l : list bool) : bool := l.foldr bxor ff
 
 namespace Xor
 
@@ -34,77 +29,39 @@ open nat
 open list
 open clause
 
-/-! # Properties -/
-
-instance : inhabited (clause V) := ⟨[arbitrary (literal V)]⟩
-instance : has_append (Xor V) := ⟨list.append⟩
-instance : has_mem (literal V) (Xor V) := ⟨list.mem⟩
-
 /-! # eval -/
 section eval
 
-variables (τ : assignment V) (g : Xor V) (l : literal V)
+variables (τ : assignment V) (l l₁ l₂ : list (literal V)) (lit : literal V)
 
 /- Evaluate the variables under the assignment according to typical XOR -/
-protected def eval : bool :=
-  g.foldr (λ l b, b ⊕ l.eval τ) ff
+protected def eval : bool := Xor (l.map (literal.eval τ))
 
 @[simp] theorem eval_nil : Xor.eval τ [] = ff := rfl
 
-@[simp] theorem eval_singleton : Xor.eval τ [l] = l.eval τ :=
-by simp only [Xor.eval, bool.bxor_ff_left, foldr]
+@[simp] theorem eval_singleton : Xor.eval τ [lit] = lit.eval τ :=
+by simp only [Xor.eval, Xor, map, bool.bxor_ff_right, foldr]
 
-theorem eval_cons : Xor.eval τ (l :: g) = bxor (l.eval τ) (g.eval τ) :=
-by simp only [Xor.eval, foldr, bool.bxor_comm]
+theorem eval_cons : Xor.eval τ (lit :: l) = bxor (lit.eval τ) (Xor.eval τ l) :=
+by simp only [Xor.eval, Xor, foldr, foldr_map]
 
-theorem eval_append (g₁ g₂ : Xor V) : 
-  Xor.eval τ (g₁ ++ g₂) = bxor (g₁.eval τ) (g₂.eval τ) :=
+theorem eval_append : 
+  Xor.eval τ (l₁ ++ l₂) = bxor (Xor.eval τ l₁) (Xor.eval τ l₂) :=
 begin
-  induction g₁ with l ls ih,
+  induction l₁ with l ls ih,
   { simp only [bool.bxor_ff_left, eval_nil, nil_append] },
   { simp only [eval_cons, ih, cons_append, bool.bxor_assoc] }
 end
 
 /- Evaluates to true if an odd number of literals evaluates to true -/
-theorem eval_eq_bodd_count_tt : g.eval τ = bodd (clause.count_tt τ g) :=
+theorem eval_eq_bodd_count_tt : Xor.eval τ l = bodd (clause.count_tt τ l) :=
 begin
-  induction g with l ls ih,
+  induction l with l ls ih,
   { simp only [bodd_zero, eval_nil, count_tt_nil] },
-  { cases h : (l.eval τ);
-    { simp [Xor.eval_cons, count_tt_cons, h, ih] } }
+  { cases h : (l.eval τ); { simp [Xor.eval_cons, count_tt_cons, h, ih] } }
 end
 
 end eval
-
-/-! # vars -/
-section vars
-
-variables {g : Xor V} {l : literal V} {v : V}
-
-/- For now, since the implementation of clause and Xor are the same,
-   using clause.lean's version of vars saves on space for redundant theorems.
-   If the implementation of clause or Xor changes, this definition will
-   need to be updated accordingly. -/
-def vars (g : Xor V) : finset V := clause.vars g
-
-@[simp] theorem vars_nil : Xor.vars ([] : Xor V) = ∅ := rfl
-
-@[simp] theorem vars_singleton (l : literal V) : Xor.vars [l] = {l.var} :=
-clause.vars_singleton l
-
-theorem mem_vars_cons_of_mem_vars : v ∈ g.vars → v ∈ Xor.vars (l :: g) :=
-clause.mem_vars_cons_of_mem_vars l
-
-theorem mem_vars_of_mem : l ∈ g → l.var ∈ g.vars :=
-clause.mem_vars_of_mem
-
-theorem vars_subset_of_vars_cons (l : literal V) (g : Xor V) :
-  g.vars ⊆ Xor.vars (l :: g) :=
-finset.subset_union_right _ _
-
--- Other theorems from clause.vars possible, if needed
-
-end vars
 
 end Xor
 
@@ -113,15 +70,16 @@ end Xor
 namespace assignment
 
 open list
+open clause
 open Xor
 
-theorem eval_eq_Xor_of_eqod {τ₁ τ₂ : assignment V} {g : Xor V} :
-  (τ₁ ≡g.vars≡ τ₂) → g.eval τ₁ = g.eval τ₂ :=
+theorem eval_eq_Xor_of_eqod {τ₁ τ₂ : assignment V} {l : list (literal V)} :
+  (τ₁ ≡(clause.vars l)≡ τ₂) → Xor.eval τ₁ l = Xor.eval τ₂ l :=
 begin
-  induction g with l ls ih,
-  { simp only [eqod_nil, eval_nil, vars_nil, forall_true_left] },
+  induction l with l ls ih,
+  { simp only [eqod_nil, Xor.eval_nil, forall_true_left, clause.vars_nil] },
   { intro h,
-    simp only [eval_cons],
+    simp only [Xor.eval_cons],
     rw eval_eq_of_eqod_of_var_mem h (mem_vars_of_mem (mem_cons_self l ls)),
     rw ih (eqod_subset (vars_subset_of_vars_cons l ls) h) }
 end
